theories/GenExtract/fintype.v
@@ -1,0 +1,368 @@
+(** * Autosubst Header for Scoped Syntax
+    Our development utilises well-scoped de Bruijn syntax. This means that the de Bruijn indices are taken from finite types. As a consequence, any kind of substitution or environment used in conjunction with well-scoped syntax takes the form of a mapping from some finite type _I^n_. In particular, _renamings_ are mappings _I^n -> I^m_. Here we develop the theory of how these parts interact.
+
+Version: December 11, 2019.
+*)
+From Undecidability Require Export axioms.
+Set Implicit Arguments.
+Unset Strict Implicit.
+
+Definition ap {X Y} (f : X -> Y) {x y : X} (p : x = y) : f x = f y :=
+  match p with eq_refl => eq_refl end.
+
+Definition apc {X Y} {f g : X -> Y} {x y : X} (p : f = g) (q : x = y) : f x = g y :=
+  match q with eq_refl => match p with eq_refl => eq_refl end end.
+
+(** ** Primitives of the Sigma Calculus
+    We implement the finite type with _n_ elements, _I^n_, as the _n_-fold iteration of the Option Type. _I^0_ is implemented as the empty type.
+*)
+
+Fixpoint fin (n : nat) : Type :=
+  match n with
+  | 0 => False
+  | S m => option (fin m)
+  end.
+
+(** Renamings and Injective Renamings
+     _Renamings_ are mappings between finite types.
+*)
+Definition ren (m n : nat) : Type := fin m -> fin n.
+
+Definition id {X} (x : X) := x.
+
+Definition idren {k: nat} : ren k k :=
+  fun x => x.
+
+(** We give a special name, to the newest element in a non-empty finite type, as it usually corresponds to a freshly bound variable. *)
+Definition var_zero {n : nat} : fin (S n) := None.
+
+Definition null {T} (i : fin 0) : T := match i with end.
+
+Definition shift {n : nat} : ren n (S n) :=
+  Some.
+
+Definition comp := @funcomp.
+
+(** Extension of Finite Mappings
+    Assume we are given a mapping _f_ from _I^n_ to some type _X_, then we can _extend_ this mapping with a new value from _x : X_ to a mapping from _I^n+1_ to _X_. We denote this operation by _x . f_ and define it as follows:
+*)
+Definition scons {X : Type} {n : nat} (x : X) (f : fin n -> X) (m : fin (S n)) : X :=
+  match m with
+  | None => x
+  | Some i => f i
+  end.
+
+
+(** ** Type Class Instances for Notation *)
+
+(** *** Type classes for renamings. *)
+
+Class Ren1 (X1  : Type) (Y Z : Type) :=
+  ren1 : X1 -> Y -> Z.
+
+Class Ren2 (X1 X2 : Type) (Y Z : Type) :=
+  ren2 : X1 -> X2 -> Y -> Z.
+
+Class Ren3 (X1 X2 X3 : Type) (Y Z : Type) :=
+  ren3 : X1 -> X2 -> X3 -> Y -> Z.
+
+Class Ren4 (X1 X2 X3 X4 : Type) (Y Z : Type) :=
+  ren4 : X1 -> X2 -> X3 -> X4 -> Y -> Z.
+
+Class Ren5 (X1 X2 X3 X4 X5 : Type) (Y Z : Type) :=
+  ren5 : X1 -> X2 -> X3 -> X4 -> X5 -> Y -> Z.
+
+Notation "s ⟨ xi1 ⟩" := (ren1  xi1 s) (at level 7, left associativity, format "s  ⟨ xi1 ⟩") : subst_scope.
+
+Notation "s ⟨ xi1 ; xi2 ⟩" := (ren2 xi1 xi2 s) (at level 7, left associativity, format "s  ⟨ xi1 ; xi2 ⟩") : subst_scope.
+
+Notation "s ⟨ xi1 ; xi2 ; xi3 ⟩" := (ren3 xi1 xi2 xi3 s) (at level 7, left associativity, format "s  ⟨ xi1 ; xi2 ; xi3 ⟩") : subst_scope.
+
+Notation "s ⟨ xi1 ; xi2 ; xi3 ; xi4 ⟩" := (ren4  xi1 xi2 xi3 xi4 s) (at level 7, left associativity, format "s  ⟨ xi1 ; xi2 ; xi3 ; xi4 ⟩") : subst_scope.
+
+Notation "s ⟨ xi1 ; xi2 ; xi3 ; xi4 ; xi5 ⟩" := (ren5  xi1 xi2 xi3 xi4 xi5 s) (at level 7, left associativity, format "s  ⟨ xi1 ; xi2 ; xi3 ; xi4 ; xi5 ⟩") : subst_scope.
+
+Notation "⟨ xi ⟩" := (ren1 xi) (at level 1, left associativity, format "⟨ xi ⟩") : fscope.
+
+Notation "⟨ xi1 ; xi2 ⟩" := (ren2 xi1 xi2) (at level 1, left associativity, format "⟨ xi1 ; xi2 ⟩") : fscope.
+
+
+(** *** Type Classes for Substiution *)
+
+Class Subst1 (X1 : Type) (Y Z: Type) :=
+  subst1 : X1 -> Y -> Z.
+
+Class Subst2 (X1 X2 : Type) (Y Z: Type) :=
+  subst2 : X1 -> X2 -> Y  -> Z.
+
+Class Subst3 (X1 X2 X3 : Type) (Y Z: Type) :=
+  subst3 : X1 -> X2 -> X3 ->  Y  -> Z.
+
+Class Subst4 (X1 X2 X3 X4: Type) (Y Z: Type) :=
+  subst4 : X1 -> X2 -> X3 -> X4 -> Y  -> Z.
+
+Class Subst5 (X1 X2 X3 X4 X5 : Type) (Y Z: Type) :=
+  subst5 : X1 -> X2 -> X3 -> X4 -> X5  -> Y  -> Z.
+
+Notation "s [ sigma ]" := (subst1 sigma s) (at level 7, left associativity, format "s '/' [ sigma ]") : subst_scope.
+
+Notation "s [ sigma ; tau ]" := (subst2 sigma tau s) (at level 7, left associativity, format "s '/' [ sigma ; '/'  tau ]") : subst_scope.
+
+(** ** Type Class for Variables *)
+Class Var X Y :=
+  ids : X -> Y.
+
+
+(** ** Proofs for substitution primitives *)
+
+(** Forward Function Composition
+    Substitutions represented as functions are ubiquitious in this development and we often have to compose them, without talking about their pointwise behaviour.
+    That is, we are interested in the forward compostion of functions, _f o g_, for which we introduce a convenient notation, "f >> g". The direction of the arrow serves as a reminder of the _forward_ nature of this composition, that is first apply _f_, then _g_. *)
+
+Arguments funcomp {X Y Z} (g)%fscope (f)%fscope.
+
+Notation "f >> g" := (funcomp g f) (at level 50).
+Open Scope subst_scope.
+
+Notation "x .: f" := (@scons _ _ x f) (at level 55) : subst_scope.
+
+(** Generic lifting operation for renamings *)
+Definition up_ren m n (xi : ren m n) : ren (S m) (S n) :=
+  var_zero .: xi >> shift.
+
+(** Generic proof that lifting of renamings composes. *)
+Lemma up_ren_ren k l m (xi: ren k l) (zeta : ren l m) (rho: ren k m) (E: forall x, (xi >> zeta) x = rho x) :
+  forall x, (up_ren xi >> up_ren zeta) x = up_ren rho x.
+Proof.
+  intros [x|].
+  - simpl. unfold funcomp. now rewrite <- E.
+  - reflexivity.
+Qed.
+
+Arguments up_ren_ren {k l m} xi zeta rho E.
+
+Lemma scons_eta {T} {n : nat} (f : fin (S n) -> T) :
+  f var_zero .: shift >> f = f.
+Proof. fext. intros [x|]; reflexivity.  Qed.
+
+
+Lemma scons_eta_id {n : nat} : var_zero .: shift = id :> (fin (S n) -> fin (S n)).
+Proof. fext. intros [x|]; reflexivity. Qed.
+
+Lemma scons_comp (T: Type) U {m} (s: T) (sigma: fin m -> T) (tau: T -> U ) :
+  (s .: sigma) >> tau = (tau s) .: (sigma >> tau) .
+Proof.
+  fext. intros [x|]. reflexivity. simpl. reflexivity.
+Qed.
+
+Lemma fin_eta {X} (f g : fin 0 -> X) :
+  forall x, f x = g x.
+Proof. intros []. Qed.
+
+
+(** ** Variadic Substitution Primitives *)
+
+Fixpoint shift_p (p : nat) {n} : ren n (p + n) :=
+  fun n => match p with
+        | 0 => n
+        | S p => Some (shift_p p n)
+        end.
+
+Fixpoint scons_p {X: Type} {m : nat} : forall {n} (f : fin m -> X) (g : fin n -> X), fin (m + n)  -> X.
+Proof.
+  destruct m.
+  - intros n f g. exact g.
+  - intros n f g. cbn. apply scons.
+    + exact (f var_zero).
+    + apply scons_p.
+      * intros z. exact (f (Some z)).
+      * exact g.
+Defined.
+
+Definition zero_p {m : nat} {n} : fin m -> fin (m + n).
+Proof.
+  induction m.
+  - intros [].
+  - intros [x|].
+    + exact (shift_p 1 (IHm x)).
+    + exact var_zero.
+Defined.
+
+Lemma scons_p_head' {X} {m n} (f : fin m -> X) (g : fin n -> X) z:
+  (scons_p  f g) (zero_p  z) = f z.
+Proof.
+ induction m.
+  - inversion z.
+  - destruct z.
+    + simpl. simpl. now rewrite IHm.
+    + reflexivity.
+Qed.
+
+Lemma scons_p_head X m n (f : fin m -> X) (g : fin n -> X) :
+  (zero_p  >> scons_p f g) = f.
+Proof. fext. intros z. unfold funcomp. apply scons_p_head'. Qed.
+
+Lemma scons_p_tail' X  m n (f : fin m -> X) (g : fin n -> X) z :
+  scons_p  f g (shift_p m z) = g z.
+Proof. induction m; cbn; eauto. Qed.
+
+Lemma scons_p_tail X  m n (f : fin m -> X) (g : fin n -> X) :
+  shift_p m  >> scons_p f g = g.
+Proof. fext. intros z. unfold funcomp. apply scons_p_tail'. Qed.
+
+Lemma destruct_fin {m n} (x : fin (m + n)):
+  (exists x', x = zero_p  x') \/ exists x', x = shift_p m x'.
+Proof.
+  induction m; simpl in *.
+  - right. eauto.
+  - destruct x as [x|].
+    + destruct (IHm x) as [[x' ->] |[x' ->]].
+      * left. now exists (Some x').
+      * right. eauto.
+    + left. exists None. eauto.
+Qed.
+
+Lemma scons_p_comp' X Y m n (f : fin m -> X) (g : fin n -> X) (h : X -> Y) x:
+ h (scons_p  f g x)  = scons_p (f >> h) (g >> h) x.
+Proof.
+  destruct (destruct_fin x) as [[x' ->]|[x' ->]].
+  - now rewrite !scons_p_head'.
+  - now rewrite !scons_p_tail'.
+Qed.
+
+Lemma scons_p_comp {X Y m n} {f : fin m -> X} {g : fin n -> X} {h : X -> Y} :
+  (scons_p f g) >> h = scons_p   (f >> h) (g >> h).
+Proof. fext. intros z. unfold funcomp. apply scons_p_comp'. Qed.
+
+Lemma scons_p_congr {X} {m n} (f f' : fin m -> X) (g g': fin n -> X) z:
+  (forall x, f x = f' x) -> (forall x, g x = g' x) -> scons_p f g z = scons_p f' g' z.
+Proof. intros H1 H2. induction m; eauto. cbn. destruct z; eauto. Qed.
+
+(** Generic n-ary lifting operation. *)
+Definition upRen_p p { m : nat } { n : nat } (xi : (fin) (m) -> (fin) (n)) : fin (p + m) -> fin (p + n)  :=
+   scons_p  (zero_p ) (xi >> shift_p _).
+
+Arguments upRen_p p {m n} xi.
+
+(** Generic proof for composition of n-ary lifting. *)
+Lemma up_ren_ren_p p k l m (xi: ren k l) (zeta : ren l m) (rho: ren k m) (E: forall x, (xi >> zeta) x = rho x) :
+  forall x, (upRen_p p xi >> upRen_p p zeta) x = upRen_p p rho x.
+Proof.
+  intros x. destruct (destruct_fin x) as [[? ->]|[? ->]].
+  - unfold upRen_p. unfold funcomp. now repeat rewrite scons_p_head'.
+  - unfold upRen_p. unfold funcomp. repeat rewrite scons_p_tail'.
+    now rewrite <- E.
+Qed.
+
+
+Arguments zero_p m {n}.
+Arguments scons_p  {X} m {n} f g.
+
+Lemma scons_p_eta {X} {m n} {f : fin m -> X}
+      {g : fin n -> X} (h: fin (m + n) -> X) {z: fin (m + n)}:
+  (forall x, g x = h (shift_p m x)) -> (forall x, f x = h (zero_p m x)) -> scons_p m f g z = h z.
+Proof.
+  intros H1 H2. destruct (destruct_fin z) as [[? ->] |[? ->]].
+  - rewrite scons_p_head'. eauto.
+  - rewrite scons_p_tail'. eauto.
+Qed.
+
+Arguments scons_p_eta {X} {m n} {f g} h {z}.
+Arguments scons_p_congr {X} {m n} {f f'} {g g'} {z}.
+
+Opaque scons.
+Opaque var_zero.
+Opaque null.
+Opaque shift.
+Opaque up_ren.
+Opaque var_zero.
+Opaque idren.
+Opaque comp.
+Opaque funcomp.
+Opaque id.
+
+
+(** ** Notations for Scoped Syntax *)
+
+Module CommaNotation.
+Notation "s , sigma" := (scons s sigma) (at level 60, format "s ,  sigma", right associativity) : subst_scope.
+End CommaNotation.
+
+Notation "s '..'" := (scons s ids) (at level 1, format "s ..") : subst_scope.
+
+Notation "↑" := (shift) : subst_scope.
+
+Ltac unfold_funcomp := match goal with
+                           | |-  context[(?f >> ?g) ?s] => change ((f >> g) s) with (g (f s))
+                           end.
+
+
+(** ** Tactics for Scoped Syntax *)
+
+(** Generic fsimpl tactic: simplifies the above primitives in a goal. *)
+Ltac fsimpl :=
+  repeat match goal with
+         | [|- context[id >> ?f]] => change (id >> f) with f (* AsimplCompIdL *)
+         | [|- context[?f >> id]] => change (f >> id) with f (* AsimplCompIdR *)
+         | [|- context [id ?s]] => change (id s) with s
+         | [|- context[comp ?f ?g]] => change (comp f g) with (g >> f) (* AsimplCompIdL *)
+         | [|- context[(?f >> ?g) >> ?h]] =>
+           change ((f >> g) >> h) with (f >> (g >> h)) (* AsimplComp *)
+
+         | [|- zero_p >> scons_p ?f ?g] => rewrite scons_p_head
+
+         | [|- context[(?s.:?sigma) var_zero]] => change ((s.:sigma) var_zero) with s
+         | [|- context[(?s.:?sigma) (shift ?m)]] => change ((s.:sigma) (shift m)) with (sigma m)
+
+         | [|- context[idren >> ?f]] => change (idren >> f) with f
+         | [|- context[?f >> idren]] => change (f >> idren) with f
+         | [|- context[?f >> (?x .: ?g)]] => change (f >> (x .: g)) with g
+         | [|- context[?x2 .: shift >> ?f]] => change x2 with (f var_zero); rewrite (@scons_eta _ _ f)
+         | [|- context[?f var_zero .: ?g]] => change g with (shift >> f); rewrite scons_eta
+
+         |[|- _ =  ?h (?f ?s)] => change (h (f s)) with ((f >> h) s)
+         |[|-  ?h (?f ?s) = _] => change (h (f s)) with ((f >> h) s)
+
+         | _ => first [progress (rewrite scons_comp) |  progress (rewrite scons_eta_id) | progress (autorewrite with FunctorInstances)]
+         end.
+
+(** Generic fsimpl tactic: simplifies the above primitives in the context *)
+Ltac fsimplc :=
+  repeat match goal with
+         | [H: context[id >> ?f] |- _] => change (id >> f) with f in H(* AsimplCompIdL *)
+         | [H: context[?f >> id]|- _] => change (f >> id) with f in H(* AsimplCompIdR *)
+         | [H: context [id ?s]|- _] => change (id s) with s in H
+         | [H: context[comp ?f ?g]|- _] => change (comp f g) with (g >> f) in H (* AsimplCompIdL *)
+         | [H: context[(?f >> ?g) >> ?h]|- _] =>
+           change ((f >> g) >> h) with (f >> (g >> h)) in H (* AsimplComp *)
+         | [H: context[(?s.:?sigma) var_zero]|- _] => change ((s.:sigma) var_zero) with s in H
+         | [H: context[(?s.:?sigma) var_zero]|- _] => change ((s.:sigma) var_zero) with s in H
+         | [H: context[(?s.:?sigma) (shift ?m)]|- _] => change ((s.:sigma) (shift m)) with (sigma m) in H
+                                                                                      |[H : context[ _ =  ?h (?f ?s)]|- _] => change (h (f s)) with ((f >> h) s) in H
+         |[H: context[?h (?f ?s) = _]|- _] => change (h (f s)) with ((f >> h) s) in H
+         | [H: context[idren >> ?f]|- _] => change (idren >> f) with f in H
+         | [H: context[?f >> idren]|- _] => change (f >> idren) with f in H
+         | [H: context[?f >> (?x .: ?g)]|- _] =>
+           change (f >> (x .: g)) with g in H
+         | [H: context[?x2 .: shift >> ?f]|- _] =>
+           change x2 with (f var_zero) in H; rewrite (@scons_eta _ _ f) in H
+         | [H: context[?f var_zero .: ?g]|- _] =>
+           change g with (shift >> f) in H; rewrite scons_eta in H
+         | _ => first [progress (rewrite scons_comp in *) | progress (rewrite scons_eta_id in *) | progress (autorewrite with FunctorInstances in *)]
+         end.
+
+(** Simplification in both the goal and the context *)
+Tactic Notation "fsimpl" "in" "*" :=
+  fsimpl; fsimplc.
+
+Tactic Notation "auto_case" tactic(t) :=  (match goal with
+                                           | [|- forall (i : fin 0), _] => intros []; t
+                                           | [|- forall (i : fin (S (S (S (S _))))), _] => intros [[[[|]|]|]|]; t
+                                           | [|- forall (i : fin (S (S (S _)))), _] => intros [[[|]|]|]; t
+                                           | [|- forall (i : fin (S (S _))), _] => intros [[?|]|]; t
+                                           | [|- forall (i : fin (S _)), _] =>  intros [?|]; t
+                                           end).
+
+
+(** Functor instances which can be added later on. *)
+Hint Rewrite  @scons_p_comp scons_p_head scons_p_tail @scons_p_head' @scons_p_tail': FunctorInstances.
