theories/GenExtract/header_extensible.v
@@ -1,0 +1,80 @@
+(** * Chapter 7 : Modular Syntax *)
+
+Require Import String List Omega.
+
+Require Import Equations.Equations.
+Set Implicit Arguments.
+Unset Strict Implicit.
+
+Arguments eq_refl {A x}, {A} x.
+
+
+(** ** Tools for modular syntax with binders *)
+
+(** *** Basic definitions  *)
+
+Lemma size_ind (P : nat -> Prop) :
+  (forall x, (forall y, y < x -> P y) -> P x) -> forall x, P x.
+Proof.
+  intros H x. apply H.
+  induction x.
+  - intros y. omega.
+  - intros y. intros [] % le_lt_or_eq.
+    + apply IHx; omega.
+    + apply H. injection H0. now intros ->.
+Qed.
+
+Class retract X Y :=
+  {
+    retract_I : X -> Y ;
+    retract_R : Y -> option X;
+    retract_works : forall x, retract_R (retract_I x) = Some x;
+    retract_tight : forall x y, retract_R y = Some x -> retract_I x = y
+  }.
+
+Arguments Build_retract {X} {Y}.
+
+Lemma retract_inj {X Y} {R : retract X Y} x y :
+  retract_I x = retract_I y -> x = y.
+Proof.
+  intros. enough (Some x = Some y) by congruence.
+  now rewrite <- !retract_works, H.
+Qed.
+
+Instance retract_option X Y : retract X Y -> retract (option X) (option Y).
+Proof.
+  intros. unshelve eexists.
+  - intros []. exact (Some (retract_I x)). exact None.
+  - intros []. destruct (retract_R y). exact (Some (Some x)). exact None. exact (Some None).
+  - intros []. cbn. now rewrite retract_works. reflexivity.
+  - intros. cbn in *. destruct y.  destruct x.
+    + destruct (retract_R y) eqn:E. inversion H. subst. clear H.
+      eapply retract_tight in E. congruence. inversion H.
+    + destruct (retract_R y) eqn:E. inversion H. inversion H.
+    + inversion H. reflexivity.
+Defined.
+
+Definition lift {X Y Y'} `{retract Y Y'} (f : X -> Y) := (fun n => retract_I (f n)).
+Notation inj := (retract_I).
+Notation retr := (retract_R).
+
+Notation included F T := (retract (F T) T)%type.
+
+Class Bundle (func : Type -> Type) (In : forall X, X -> func X -> Prop) := make_Bundle {}.
+Existing Instance make_Bundle.
+
+Definition get_In {func In} {bundle : @Bundle func In} := In.
+
+Lemma congr_inj {X Y} `{retract X Y} {x y}:
+  x = y -> inj x = inj y.
+Proof.
+  congruence.
+Qed.
+
+Lemma Some_inj {X} {x y : X} :
+  Datatypes.Some x = Datatypes.Some y -> x = y.
+Proof. congruence. Qed.
+
+Lemma some_none_explosion {X : Type} {x : X} {H : Prop} :
+  Datatypes.None = Datatypes.Some x  -> H.
+Proof. intros A. congruence. Qed.
